Add partiality to the maps

src/Std/Data/DHashMap/Internal/Defs.lean
@@ -4,6 +4,7 @@ Released under Apache 2.0 license as described in the file LICENSE.
 Authors: Leonardo de Moura, Mario Carneiro, Markus Himmel
 -/
 prelude
+import Init.Data.Array.Attach
 import Init.Data.Array.Lemmas
 import Std.Data.DHashMap.RawDef
 import Std.Data.Internal.List.Defs
@@ -407,11 +408,12 @@ where
   ⟨⟨size, newBuckets⟩, by simpa [newBuckets] using hb⟩
 
 /-- Internal implementation detail of the hash map -/
-@[inline] def mapKeyValueInPlace
-    (f : (a : α) → β a → ((a' : α') × β' a'))
-    (m : Raw₀ α β) : Raw₀ α' β' :=
+@[inline] def pmapEntries {P : (a : α) → (b : β a) → Prop}
+    (f : (a : α) → (b : β a) → P a b → ((a' : α') × β' a'))
+    (m : Raw₀ α β) (H : ∀ a b, ⟨a, b⟩ ∈ toListModel m.val.buckets → P a b) : Raw₀ α' β' :=
   let ⟨⟨size, buckets⟩, hb⟩ := m
-  let newBuckets := buckets.map (AssocList.mapKeyValue f)
+  let newBuckets := buckets.attach.map λ ⟨bucket, hb⟩ ↦
+     AssocList.pmapEntries f bucket (fun a b h => H a b (List.mem_flatMap.mpr ⟨bucket, hb.val, h⟩))
   ⟨⟨size, newBuckets⟩, by simpa [newBuckets] using hb⟩
 
 /-- Internal implementation detail of the hash map -/
